mechanization/HADL/Typing.lean
@@ -38,7 +38,7 @@ inductive RtType : Env → Value → Ty → Prop where
   /-- Resolution through ρ: if the type name `y` is bound to a schema value
       `vSchema τ'`, then runtime typing against `tVar y` unfolds to τ'. -/
   | tVarResolve {ρ y τ' v} :
-      (Env.lookup ρ y) = some ⟨.vSchema τ', .tSchema, none, .letBind⟩ →
+      (Env.lookup ρ y) = some ⟨.vSchema τ', .tSchema, .letBind⟩ →
       RtType ρ v τ' →
       RtType ρ v (.tVar y)
 
